

Convex Programming

Problem Set 5 – CS 6515/4540 (Fall 2025)

This problem set is due on **Tuesday November 4th**. Submission is via Gradescope. Your solution must be a typed pdf (e.g. via LaTeX) – no handwritten solutions.

18 Convex Functions

1. Given two convex functions $f : \mathbb{R} \rightarrow \mathbb{R}$ and $g : \mathbb{R} \rightarrow \mathbb{R}$, is the sum $f + g$ also convex? Either prove it or give a counterexample.

Yes, because

$$\begin{aligned}(f + g)(\lambda x + (1 - \lambda)y) &= f(\lambda x + (1 - \lambda)y) + g(\lambda x + (1 - \lambda)y) \\ &\leq \lambda f(x) + (1 - \lambda)f(y) + \lambda g(x) + (1 - \lambda)g(y) = \lambda(f(x) + g(x)) + (1 - \lambda)(f(y) + g(y))\end{aligned}$$

and so we're done.

2. Given two convex functions $f : \mathbb{R} \rightarrow \mathbb{R}$ and $g : \mathbb{R} \rightarrow \mathbb{R}$, is the product fg also convex? Either prove it or give a counterexample.

No, consider $f(x) = -1$ and $g(x) = x^2$. Both are convex but $fg = -x^2$ is not convex.

3. What about the convexity of the function $h : \mathbb{R} \rightarrow \mathbb{R}$ defined by $h(x) = \max(f(x), g(x))$? Prove it or give a counterexample.

Yes,

$$\begin{aligned}h(\lambda x + (1 - \lambda)y) &= \max(f(\lambda x + (1 - \lambda)y), g(\lambda x + (1 - \lambda)y)) \\ &\leq \max(\lambda f(x) + (1 - \lambda)f(y), \lambda g(x) + (1 - \lambda)g(y)) \leq \lambda h(x) + (1 - \lambda)h(y)\end{aligned}$$

where the last step follows from the fact that $f(x) \leq h(x)$, $g(x) \leq h(x)$ for all x .

4. Show an α -strongly convex function (defined in Pb 20) $f : \mathbb{R} \rightarrow \mathbb{R}$ satisfies $f(x) = \Omega(x^2)$

Simply plug in $x = x^*$, where x^* is the unique minimum of f where $\nabla f(x^*) = 0$, and then it is quite obvious we have a quadratic via the definition of strong convexity:

$$f(y) \geq f(x^*) + \frac{\alpha}{2}(y - x^*)^2$$

Since x^* is a constant, the above equation is a quadratic in y , showing that f grows at least as fast as a quadratic.

19 Gradient Descent Failure

Suppose we run an unconstrained Gradient Descent on $f(x) = \frac{1}{2}x^2$ with some arbitrary step size. Give (and justify) an example consisting of

1. a step size $\eta > 0$
2. an initial point $x_0 \in \mathbb{R}$

such that t -th **average** $\bar{x}_t = \frac{1}{t} \sum_{i \leq t} x_i$ of an unconstrained Gradient Descent with the above parameters does not converge (e.g it diverges) to the optimum as $t \rightarrow \infty$.

Example

We provide the following example:

$$\eta = 3 \tag{1}$$

$$x_0 = 1 \tag{2}$$

More generally, any step size $\eta > 2$ with any initial point $x_0 \neq 0$ will cause the average to diverge.

Setup and Gradient Descent Update

For the function $f(x) = \frac{1}{2}x^2$, we have:

- Gradient: $\nabla f(x) = x$
- Optimum: $x^* = 0$ with $f(x^*) = 0$
- GD update rule: $x_{t+1} = x_t - \eta \nabla f(x_t) = x_t - \eta x_t = (1 - \eta)x_t$

Computing the Average

The t -th average is:

$$\bar{x}_t = \frac{1}{t} \sum_{i=0}^{t-1} x_i = \frac{1}{t} \sum_{i=0}^{t-1} (1 - \eta)^i x_0 = \frac{x_0}{t} \sum_{i=0}^{t-1} (1 - \eta)^i \tag{3}$$

Using the geometric series formula (assuming $\eta \neq 0$):

$$\sum_{i=0}^{t-1} r^i = \frac{1 - r^t}{1 - r} \tag{4}$$

we obtain:

$$\bar{x}_t = \frac{x_0}{t} \cdot \frac{1 - (1 - \eta)^t}{1 - (1 - \eta)} = \frac{x_0}{t\eta} [1 - (1 - \eta)^t] \tag{5}$$

Analysis of Convergence

Case 1: $0 < \eta < 2$ (Standard Convergent Regime)

In this case, $|1 - \eta| < 1$, so $(1 - \eta)^t \rightarrow 0$ as $t \rightarrow \infty$. Therefore:

$$\bar{x}_t = \frac{x_0}{t\eta} [1 - (1 - \eta)^t] \rightarrow \frac{x_0}{t\eta} \rightarrow 0 \tag{6}$$

The average converges to the optimum $x^* = 0$.

Case 2: $\eta = 2$ (Boundary Case)

Here, $1 - \eta = -1$, so the iterates oscillate:

$$x_t = (-1)^t x_0 \quad (7)$$

The sequence is $x_0, -x_0, x_0, -x_0, \dots$

For the average:

- If t is even: $\bar{x}_t = 0$ (equal numbers of $+x_0$ and $-x_0$)
- If t is odd: $\bar{x}_t = \frac{x_0}{t} \rightarrow 0$

Therefore, $\bar{x}_t \rightarrow 0$. The average still converges despite the oscillation of individual iterates.

Case 3: $\eta > 2$ (Divergent Regime)

This is the regime where the average diverges.

For $\eta > 2$, we have $1 - \eta < -1$, so $|1 - \eta| > 1$. Let $r = 1 - \eta$ with $|r| > 1$. Then:

$$\bar{x}_t = \frac{x_0}{t\eta} (1 - r^t) = \frac{x_0}{t\eta} - \frac{x_0 r^t}{t\eta} \quad (8)$$

As $t \rightarrow \infty$, the term $\frac{x_0 r^t}{t\eta}$ behaves as:

$$\frac{|r|^t}{t} \rightarrow \infty \quad (9)$$

This is because exponential growth $|r|^t$ dominates polynomial growth t . More formally, for $|r| > 1$:

$$\lim_{t \rightarrow \infty} \frac{|r|^t}{t} = \lim_{t \rightarrow \infty} \frac{e^{t \ln |r|}}{t} = \infty \quad (10)$$

Therefore, $|\bar{x}_t| \rightarrow \infty$, and the average diverges. For this specific example:

- $1 - \eta = 1 - 3 = -2$
- $x_t = (-2)^t$
- Iterates: $1, -2, 4, -8, 16, -32, \dots$

The average is:

$$\bar{x}_t = \frac{1 - (-2)^t}{3t} = \frac{1}{3t} - \frac{(-2)^t}{3t} \quad (11)$$

For large t :

$$|\bar{x}_t| \approx \frac{2^t}{3t} \rightarrow \infty \quad (12)$$

The average diverges to $\pm\infty$ (oscillating in sign). The step size $\eta = 3$ causes the algorithm to overshoot dramatically:

- Each iteration, we move by $\eta x_t = 3x_t$
- This takes us to $x_{t+1} = x_t - 3x_t = -2x_t$
- We overshoot the optimum and end up twice as far on the opposite side
- The magnitude grows exponentially: $|x_t| = 2^t$

Even though we're averaging, the exponential growth overwhelms the $1/t$ decay from averaging, causing divergence.

Note that if $x_0 = 0$ (starting at the optimum), then $x_t = 0$ for all t regardless of η , and the average trivially remains at the optimum. Therefore, any valid example must have $x_0 \neq 0$.

20 Gradient Descent for Strongly-Convex Functions

A differentiable function f is α -strongly convex for $\alpha > 0$ if for all $x, y \in \mathbb{R}^n$ we have

$$f(y) \geq f(x) + \langle \nabla f(x), y - x \rangle + \frac{\alpha}{2} \|y - x\|_2^2.$$

Consider an α -strongly convex differentiable function f with the 2-norm of its gradient always bounded by G . The goal is to minimize f and let x^* denote its minimum.

Show that the gradient descent algorithm with step size $\frac{1}{\alpha(t+1)}$ satisfies

$$f\left(\frac{\sum_t x_t}{T}\right) - f(x^*) \leq \frac{G^2(1 + \log T)}{2\alpha T}.$$

Thus, strong-convexity allows us to get $1/T$ dependency in regret instead of $1/\sqrt{T}$ dependency for general convex functions.

(Hint: Change the potential function in the analysis from class to $\Phi(t) = \frac{t\alpha}{2} \|x_t - x^*\|^2$. Also, use that $\sum_{t \in \{1, \dots, T\}} \frac{1}{t} \leq 1 + \log T$.)

Let n be the step size and f be our feedback function. Consider the potential function $\Phi(t) = \frac{\alpha t}{2} \|x_t - x^*\|^2$. Note that $\|y_{t+1} - x^*\|^2 \geq \|x_{t+1} - x^*\|^2$ by the lecture notes (projection on K). Using this, as well as our step size $n = \frac{1}{\alpha(t+1)}$ and the upper bound on our gradient (G) along with the definition of α -strong convexity,

$$\begin{aligned} \Phi(t+1) &= \frac{\alpha(t+1)}{2} (\|x_{t+1} - x^*\|^2) \leq \frac{\alpha(t+1)}{2} (\|y_{t+1} - x^*\|^2) = \frac{\alpha(t+1)}{2} \|x_t - x^* - n\nabla f(x_t)\|^2 \\ &= \frac{\alpha(t+1)}{2} (\|x_t - x^*\|^2 + (n\nabla f(x_t))^2 - 2n\langle x_t - x^*, \nabla f(x_t) \rangle) \\ &= \Phi(t) + \frac{\alpha}{2} \|x_t - x^*\|^2 + \frac{(\nabla f(x_t))^2}{2\alpha(t+1)} - \langle x_t - x^*, \nabla f(x_t) \rangle \\ &\leq \Phi(t) + f(x^*) - f(x_t) + \frac{G^2}{2\alpha(t+1)} \\ \implies f(x_t) - f(x^*) &\leq \Phi(t) - \Phi(t+1) + \frac{G^2}{2\alpha(t+1)} \\ \implies \sum_t f(x_t) - f(x^*) &\leq \Phi(0) - \Phi(T+1) + \frac{G^2}{2\alpha} \sum_t \frac{1}{t+1} \leq \frac{G^2(1 + \log(T))}{2\alpha} \end{aligned}$$

where the last step utilizes the observations that $\Phi(0) - \Phi(t+1) \leq 0$, and $\sum_t \frac{1}{t} \leq 1 + \log(T)$. Applying convexity to the left hand side, we have $f\left(\frac{\sum_t x_t}{T}\right) - f(x^*) \leq \frac{G^2(1 + \log(T))}{2\alpha T}$ and we are done.

21 Non-Convex Function

In class we assumed function f is convex. We now want to consider the non-convex case. We want to show that for L -smooth f , after t iterations with step size $\eta \leq 1/L$ we can find a point x' with

$$\|\nabla f(x')\| \leq \sqrt{\frac{2}{\eta \cdot t} (f(x^0) - f(x^*))}.$$

(Note that for a local optimum we have $\nabla f(x) = 0$, so a small norm $\|\nabla f(x')\|$ indicates that we are close to a local optimum or saddle point.)

Proving this from scratch is a bit tricky, so we provide the following subproblems to guide you to a proof. Each subproblem can be solved in a few lines of calculation/algebra.

Problem:

1. Show $f(x^{t+1}) \leq f(x^t) - \frac{\eta}{2} \|\nabla f(x^t)\|^2$ (Hint: Check the proof from class for convex functions. Does it work for non-convex functions?)
2. Show $\sum_{k=0}^t \|\nabla f(x^k)\|^2 \leq \frac{2}{\eta} (f(x^0) - f(x^*))$ (Hint: 1. implies $\frac{\eta}{2} \|\nabla f(x^t)\|^2 \leq \dots$)
3. Show $\min_{k=0\dots t} \|\nabla f(x^k)\| \leq \sqrt{\frac{2}{\eta \cdot t} (f(x^0) - f(x^*))}$.

where x^* is the global optimum $f(x^*) = \min_x f(x)$.

You are allowed to use subproblems to solve later subproblems (e.g., use 1+2 to solve 3), even if you did not prove them.

1. This property has already been proven in class, and actually follows from L -smoothness alone; it does not require convexity of function f . The proof is repeated here for completeness:

For an L -smooth function, from the lemma in lectures, we have:

$$|f(y) - (f(x) + \nabla f(x)^\top (y - x))| \leq \frac{L}{2} \|y - x\|^2 \Rightarrow f(y) \leq f(x) + \nabla f(x)^\top (y - x) + \frac{L}{2} \|y - x\|^2$$

Substituting in $y = x^{t+1} = x^t - \eta \nabla f(x)$ (for $\eta \leq 1/L$), and $x = x^t$ in the above, we get:

$$\begin{aligned} f(x^{t+1}) &\leq f(x^t) + \nabla f(x^t)^\top (x^t - \eta \nabla f(x) - x^t) + \frac{L}{2} \|x^t - \eta \nabla f(x) - x^t\|^2 \\ &= f(x^t) - \eta \nabla f(x^t)^\top \nabla f(x) + \frac{L}{2} \|\eta \nabla f(x^t)\|^2 \\ &= f(x^t) - \eta \|\nabla f(x^t)\|^2 + \frac{L\eta^2}{2} \|\nabla f(x^t)\|^2 \\ &\leq f(x^t) - \eta \|\nabla f(x^t)\|^2 + \frac{\eta}{2} \|\nabla f(x^t)\|^2 \quad (\text{since } L \leq 1/\eta) \\ &= f(x^t) - \frac{\eta}{2} \|\nabla f(x^t)\|^2 \end{aligned}$$

2. Rearranging the result of part 1, we get:

$$\|\nabla f(x^k)\|^2 \leq \frac{2}{\eta} [f(x^k) - f(x^{k+1})]$$

The above inequality holds for all t . So, summing over all $k = 0, \dots, t$, we get:

$$\sum_{k=0}^t \|\nabla f(x^k)\|^2 \leq \sum_{k=0}^t \frac{2}{\eta} [f(x^k) - f(x^{k+1})] = \frac{2}{\eta} [f(x^0) - f(x^{t+1})]$$

In the above, the equality follows from the fact that the summation telescopes (part of previous terms in the summation cancel with part of future terms). Now, by definition of $x^* = \operatorname{argmin}_x f(x)$, we have $f(x^*) \leq f(x^{t+1}) \Leftrightarrow -f(x^*) \leq -f(x^{t+1})$. As a result, we get:

$$\sum_{k=0}^t \|\nabla f(x^k)\|^2 \leq \frac{2}{\eta} [f(x^0) - f(x^*)]$$

3. Dividing the inequality obtained from part 2 by 2, we have:

$$\frac{1}{t} \sum_{k=0}^t \|\nabla f(x^k)\|^2 \leq \frac{2}{\eta \cdot t} [f(x^0) - f(x^*)]$$

Since the average of a set of numbers is at least the minimum among the set, we have the relation:

$$\min_{k=0 \dots t} \|\nabla f(x^k)\|^2 \leq \frac{1}{t} \sum_{k=0}^t \|\nabla f(x^k)\|^2$$

Therefore, we conclude:

$$\min_{k=0 \dots t} \|\nabla f(x^k)\|^2 \leq \frac{2}{\eta \cdot t} [f(x^0) - f(x^*)] \Leftrightarrow \min_{k=0 \dots t} \|\nabla f(x^k)\| \leq \sqrt{\frac{2}{\eta \cdot t} [f(x^0) - f(x^*)]}$$